In preparation for adding ARM's Thumb instructions - the ISA model has been updated from version 3M to version 4.  Therefore:
* There is a new mode (sys).

* Data transfers for signed/unsigned half words and signed bytes have
  been added.  (LDRSB, LDRSH, LDRH and STRH).

A number of changes have been made:

* DECODE_INST is now called DECODE_ARM and it is now defined using
  a case expression.

* The type :transfer_options has dropped the component "BSN".  Instead,
  there is a new bool element for the constructors LDR, STR, LDM, STM,
  LDC and STC.

* More use has been made of case expressions i.e. in the definition
  of RUN_ARM and OUT_ARM.

To support coprocessors, a couple of other changes have been made:

* The output now includes a component CPI, which is true when a
  coprocessor instruction is being run.

* The CPMemRead and CPMemWrite constructors have been dropped.

* TRANSFERS has a new definition.

examples/elliptic/arm/Data.sml
@@ -22,6 +22,10 @@ datatype addr_mode2 =
    DtImmediate of int
  | DtShiftImmediate of {Imm : int, Rm : vregister, Sh : shift};
 
+datatype addr_mode3 =
+   DthImmediate of int
+ | DthRegister of vregister;
+
 datatype msr_mode = MsrImmediate of Arbnum.num | MsrRegister of vregister;
 
 datatype ARM_instruction =
@@ -31,6 +35,8 @@ datatype ARM_instruction =
                   op2 : addr_mode1}
   | Mla_mul of {L : bool, Signed : bool, A : bool, S : bool, Rd : vregister,
                 Rn : vregister, Rs : vregister, Rm : vregister}
+  | Ldrh_strh of {P : bool, U : bool, W : bool, L : bool, S : bool, H : bool,
+                  Rn : vregister, Rd : vregister, offset : addr_mode3}
   | Ldr_str of {P : bool, U : bool, B : bool, W : bool, L : bool,
                 Rn : vregister, Rd : vregister, offset : addr_mode2}
   | Ldm_stm of {P : bool, U : bool, S : bool, W : bool, L : bool,
