examples/elliptic/arm/bsubstScript.sml
@@ -57,9 +57,39 @@ val _ = computeLib.auto_import_definitions := true;
 
 (* ------------------------------------------------------------------------- *)
 
+val _ = Hol_datatype
+  `formats = SignedByte | UnsignedByte
+           | SignedHalfWord | UnsignedHalfWord
+           | UnsignedWord`;
+
+val _ = Hol_datatype
+  `data = Byte of word8 | Half of word16 | Word of word32`;
+
 val _ = type_abbrev("mem", ``:word30->word32``);
 
-val ADDR30_def = Define `ADDR30 (addr:word32) = (31 >< 2) addr:word30`;
+val GET_BYTE_def = Define`
+  GET_BYTE (oareg:word2) (data:word32) =
+    (case oareg of
+        0w -> (7 >< 0) data
+     || 1w -> (15 >< 8) data
+     || 2w -> (23 >< 16) data
+     || _  -> (31 >< 24) data):word8`;
+
+val GET_HALF_def = Define`
+  GET_HALF (oareg:word2) (data:word32) =
+    (if oareg %% 1 then
+       (31 >< 16) data
+     else
+       (15 >< 0) data):word16`;
+
+val FORMAT_def = Define`
+  FORMAT fmt oareg data =
+    case fmt of
+       SignedByte       -> sw2sw (GET_BYTE oareg data)
+    || UnsignedByte     -> w2w (GET_BYTE oareg data)
+    || SignedHalfWord   -> sw2sw (GET_HALF oareg data)
+    || UnsignedHalfWord -> w2w (GET_HALF oareg data)
+    || UnsignedWord     -> data`;
 
 val SET_BYTE_def = Define`
   SET_BYTE (oareg:word2) (b:word8) (w:word32) =
@@ -69,16 +99,33 @@ val SET_BYTE_def = Define`
       (16 <= i /\ i < 24) /\ (if oareg = 2w then b %% (i - 16) else x) \/
       (24 <= i /\ i < 32) /\ (if oareg = 3w then b %% (i - 24) else x)) w`;
 
+val SET_HALF_def = Define`
+  SET_HALF (oareg:bool) (hw:word16) (w:word32) =
+    word_modify (\i x.
+                 (i < 16) /\ (if ~oareg then hw %% i else x) \/
+      (16 <= i /\ i < 32) /\ (if oareg then hw %% (i - 16) else x)) w`;
+
+val ADDR30_def = Define `ADDR30 (addr:word32) = (31 >< 2) addr:word30`;
+
 val MEM_WRITE_BYTE_def = Define`
-  MEM_WRITE_BYTE (mem:mem) addr (word:word32) =
+  MEM_WRITE_BYTE (mem:mem) addr (word:word8) =
     let addr30 = ADDR30 addr in
-      (addr30 :- SET_BYTE ((1 >< 0) addr) ((7 >< 0) word) (mem addr30)) mem`;
+      (addr30 :- SET_BYTE ((1 >< 0) addr) word (mem addr30)) mem`;
+
+val MEM_WRITE_HALF_def = Define`
+  MEM_WRITE_HALF (mem:mem) addr (word:word16) =
+    let addr30 = ADDR30 addr in
+      (addr30 :- SET_HALF (addr %% 1) word (mem addr30)) mem`;
 
 val MEM_WRITE_WORD_def = Define`
   MEM_WRITE_WORD (mem:mem) addr word = (ADDR30 addr :- word) mem`;
 
 val MEM_WRITE_def = Define`
-  MEM_WRITE b = if b then MEM_WRITE_BYTE else MEM_WRITE_WORD`;
+  MEM_WRITE mem addr d =
+    case d of
+       Byte b  -> MEM_WRITE_BYTE mem addr b
+    || Half hw -> MEM_WRITE_HALF mem addr hw
+    || Word w  -> MEM_WRITE_WORD mem addr w`;
 
 val MEM_READ_def        = Define`MEM_READ (m: mem, a) = m a`;
 val MEM_WRITE_BLOCK_def = Define`MEM_WRITE_BLOCK (m:mem) a c = (a ::- c) m`;
@@ -194,19 +241,27 @@ val _ = let open EmitML in emitML (!Globals.emitMLDir)
          :: MLSIG "type num = numML.num"
          :: MLSIG "type word2 = wordsML.word2"
          :: MLSIG "type word8 = wordsML.word8"
+         :: MLSIG "type word16 = wordsML.word16"
          :: MLSIG "type word30 = wordsML.word30"
          :: MLSIG "type word32 = wordsML.word32"
          :: MLSTRUCT "type mem = word30->word32"
          :: MLSIG "type mem"
          :: MLSTRUCT "val mem_updates = ref ([]: word30 list)"
          :: MLSIG "val mem_updates : word30 list ref"
+         :: DATATYPE (`formats = SignedByte | UnsignedByte
+                               | SignedHalfWord | UnsignedHalfWord
+                               | UnsignedWord`)
+         :: DATATYPE (`data = Byte of word8 | Half of word16 | Word of word32`)
          :: map (DEFN o BETA_RULE o PURE_REWRITE_RULE
-             [GSYM n2w_itself_def, GSYM w2w_itself_def,
+             [GSYM n2w_itself_def, GSYM w2w_itself_def, GSYM sw2sw_itself_def,
               GSYM word_extract_itself_def] o
              RHS_REWRITE_RULE [GSYM word_eq_def])
-           [SUBST_def, BSUBST_def, ADDR30_def, SET_BYTE_def, MEM_READ_def,
-            mem_read_rule MEM_WRITE_BYTE_def, MEM_WRITE_WORD_def, MEM_WRITE_def,
-            MEM_WRITE_BLOCK_def, MEM_ITEMS_def, empty_memory_def])
+           [SUBST_def, BSUBST_def, GET_HALF_def,
+            SIMP_RULE std_ss [literal_case_DEF] GET_BYTE_def,
+            FORMAT_def, ADDR30_def, SET_BYTE_def, SET_HALF_def,
+            MEM_READ_def, MEM_ITEMS_def, empty_memory_def,
+            mem_read_rule MEM_WRITE_BYTE_def, mem_read_rule MEM_WRITE_HALF_def,
+            MEM_WRITE_WORD_def, MEM_WRITE_def, MEM_WRITE_BLOCK_def])
 end;
 
 (* ------------------------------------------------------------------------- *)
